Loom/Lawful/Lift.lean
@@ -9,8 +9,8 @@ section MonadLift
 class LawfulWPMonadLift
     (m : semiOutParam (Type u → Type v)) (l : semiOutParam (Type w)) (e : semiOutParam (Type z))
     (n : Type u → Type v') (k : Type w') (d : Type z')
-    [Monad m] [CompleteLattice l] [CompleteLattice e] [WPMonad m l e]
-    [Monad n] [CompleteLattice k] [CompleteLattice d] [WPMonad n k d]
+    [Monad m] [WPMonad m l e]
+    [Monad n] [WPMonad n k d]
     [inst : MonadLift m n] [inst' : MonadLift (PredTrans l e) (PredTrans k d)] : Prop where
   /-- Lifting preserves `wp` -/
   lift_wp_trans {α : Type u} (x : m α) : inst'.monadLift (wpTrans x) ⊑ wpTrans (inst.monadLift x)
@@ -22,8 +22,8 @@ class LawfulWPMonadLift
 class LawfulWPMonadLiftT
     (m : Type u → Type v) (l : Type w) (e : Type z)
     (n : Type u → Type v') (k : Type w') (d : Type z')
-    [Monad m] [CompleteLattice l] [CompleteLattice e] [WPMonad m l e]
-    [Monad n] [CompleteLattice k] [CompleteLattice d] [WPMonad n k d]
+    [Monad m] [WPMonad m l e]
+    [Monad n] [WPMonad n k d]
     [inst : MonadLiftT m n] [inst' : MonadLiftT (PredTrans l e) (PredTrans k d)] : Prop where
   /-- Lifting preserves `wp` -/
   lift_wp_trans {α : Type u} (x : m α) : inst'.monadLift (wpTrans x) ⊑ wpTrans (inst.monadLift x)
@@ -34,7 +34,7 @@ class LawfulWPMonadLiftT
 export LawfulWPMonadLiftT (lift_wp_trans lift_monotone)
 
 instance (m : Type u → Type v) (l : Type w) (e : Type z) (σ : Type u)
-  [Monad m] [CompleteLattice l] [CompleteLattice e] [WPMonad m l e] :
+  [Monad m] [WPMonad m l e] :
   LawfulWPMonadLift m l e (StateT σ m) (σ → l) e where
   lift_wp_trans x := fun post epost s => by
     simp only [MonadLift.monadLift]
@@ -46,13 +46,13 @@ instance (m : Type u → Type v) (l : Type w) (e : Type z) (σ : Type u)
   lift_monotone _ _ h := fun post epost s => h (fun a => post a s) epost
 
 instance (m : Type u → Type v) (l : Type w) (e : Type z) (ρ : Type u)
-  [Monad m] [CompleteLattice l] [CompleteLattice e] [WPMonad m l e] :
+  [Monad m] [WPMonad m l e] :
   LawfulWPMonadLift m l e (ReaderT ρ m) (ρ → l) e where
   lift_wp_trans _x := fun _post _epost _r => PartialOrder.rel_refl
   lift_monotone _ _ h := fun post epost r => h (fun a => post a r) epost
 
 instance (m : Type u → Type v) (l : Type w) (e : Type z) (ε : Type u)
-  [Monad m] [CompleteLattice l] [CompleteLattice e] [WPMonad m l e] :
+  [Monad m] [WPMonad m l e] :
   LawfulWPMonadLift m l e (ExceptT ε m) l (EPost.cons (ε → l) e) where
   lift_wp_trans x := fun post epost => by
     simp only [MonadLift.monadLift, ExceptT.lift, ExceptT.mk]
@@ -67,7 +67,7 @@ variable {m : Type u → Type v} {n : Type u → Type w} {o : Type u → Type x}
 -- analogue of instLawfulMonadLiftT (reflexive)
 instance
     {l : Type w'} {e : Type z'}
-    [CompleteLattice l] [CompleteLattice e] [Monad m] [WPMonad m l e] :
+    [Monad m] [WPMonad m l e] :
     LawfulWPMonadLiftT m l e m l e where
   lift_wp_trans _x := fun _post _epost => PartialOrder.rel_refl
   lift_monotone _ _ h := h
@@ -75,9 +75,9 @@ instance
 -- analogue of instLawfulMonadLiftTOfLawfulMonadLift (transitive)
 instance
     {l : Type w'} {e : Type z'} {k : Type w''} {d : Type z''} {p : Type w'''} {c : Type z'''}
-    [CompleteLattice l] [CompleteLattice e] [Monad m] [WPMonad m l e]
-    [CompleteLattice k] [CompleteLattice d] [Monad n] [WPMonad n k d]
-    [CompleteLattice p] [CompleteLattice c] [Monad o] [WPMonad o p c]
+    [Monad m] [WPMonad m l e]
+    [Monad n] [WPMonad n k d]
+    [Monad o] [WPMonad o p c]
     [MonadLiftT m n] [MonadLiftT (PredTrans l e) (PredTrans k d)]
     [MonadLift n o] [MonadLift (PredTrans k d) (PredTrans p c)]
     [LawfulWPMonadLift n k d o p c] [LawfulWPMonadLiftT m l e n k d] :
